problems/4/Problem4.dfy
@@ -1,9 +1,134 @@
+include "../../parser/split.dfy"
+include "../../parser/parseInt.dfy"
 module Problem4 {
-    method problem4_1(input: string) returns (x: int) {
-        return 3;
+    import opened Split
+    method parseInput(input: string) returns (grid: seq<string>, n: nat)
+        ensures |grid| > 0
+        ensures forall i :: 0 <= i < |grid| ==> |grid[i]| == n
+    {
+        grid := splitOnBreak(input);
+        expect |grid| > 0;
+        n := |grid[0]|;
+        expect forall i :: 0 <= i < |grid| ==> |grid[i]| == n;
     }
 
-    method problem4_2(input: string) returns (x: int) {
-        return 4;
+    function adjacentIndexes(): set<(int, int)> {
+        (set i: int,j: int | -1 <= i <= 1 && -1 <= j <= 1 :: (i,j)) - {(0,0)}
+    }
+
+    predicate LteTuple(a: (int, int), b: (int, int)) {
+        if a.0 < b.0 then
+            true
+        else if a.0 > b.0 then
+            false
+        else if a.1 <= b.1 then
+            true
+        else
+            false
+    }
+
+    lemma ThereIsAMinimum(s: set<(int, int)>)
+        requires s != {}
+        ensures exists x :: x in s && forall y :: y in s ==> LteTuple(x, y)
+    {
+        assert s != {};
+        var x :| x in s;
+        if s == {x} {
+        } else {
+            var s' := s - {x};
+            assert s == s' + {x};
+            ThereIsAMinimum(s');
+        }
+    }
+
+    function SetToSequence(s: set<(int,int)>): seq<(int,int)>
+        ensures var q := SetToSequence(s); forall i :: 0 <= i < |q| ==> q[i] in s
+        ensures |SetToSequence(s)| == |s|
+        ensures forall p :: p in s ==> p in SetToSequence(s)
+    {
+    if s == {} then [] else
+        ThereIsAMinimum(s);
+        var x :| x in s && forall y :: y in s ==> LteTuple(x, y);
+        [x] + SetToSequence(s - {x})
+    }
+
+
+    const Offsets: seq<(int,int)> := SetToSequence(adjacentIndexes())
+
+    function neighbors(grid: seq<string>, x: nat, y: nat, n: nat, offsets: seq<(int, int)>, removed: set<(nat,nat)>): multiset<char> 
+        requires forall i :: 0 <= i < |grid| ==> |grid[i]| == n
+        requires y < |grid|
+        requires x < |grid[y]|
+    {
+        if offsets == [] then multiset{}
+        else 
+            var offset := offsets[0];
+            if 0 <= y+offset.1 < |grid| && 0 <= x+offset.0 < |grid[y+offset.1]| && (x+offset.0, y+offset.1) !in removed then
+                multiset{grid[y+offset.1][x+offset.0]} + neighbors(grid, x, y, n, offsets[1..], removed)
+            else
+                neighbors(grid, x, y, n, offsets[1..], removed)
+    }
+
+    predicate ltFour(grid: seq<string>, x: nat, y: nat, n: nat, removed: set<(nat,nat)>)
+        requires forall i :: 0 <= i < |grid| ==> |grid[i]| == n
+        requires y < |grid|
+        requires x < |grid[y]|
+    {
+        neighbors(grid, x, y, n, Offsets, removed)['@'] < 4
+    }
+
+    method problem4_1(input: string) returns (x: int) {
+       var grid, length := parseInput(input);
+       x := 0;
+       print "indices", Offsets;
+       var removed: set<(nat,nat)> := {};
+       for i := 0 to |grid| {
+           for k := 0 to length {
+                if ltFour(grid, k, i, length, removed) && grid[i][k] == '@' {
+                    // print "\n(", k, ", ", i, ")";
+                    x := x + 1;
+                }
+           }
+       }
+    }
+
+    method problem4_helper(grid: seq<string>, length: nat, removed: set<(nat,nat)>) returns (x: int, removed': set<(nat,nat)>)
+        requires forall i :: 0 <= i < |grid| ==> |grid[i]| == length
+    {
+       x := 0;
+       var found: set<(nat, nat)> := {};
+       for i := 0 to |grid|
+            invariant x == |found|
+            invariant forall index :: index in found ==> index.1 < i
+       {
+           for k := 0 to length 
+                invariant x == |found|
+                invariant forall index :: index in found ==> index.1 <= i
+                invariant forall index :: index in found ==> index.0 >= k ==> index.1 < i
+           {
+                if ltFour(grid, k, i, length, removed) && grid[i][k] == '@' && (k,i) !in removed {
+                    assert (k,i) !in found;
+                    found := found + {(k,i)};
+                    x := x + 1;
+                }
+           }
+       }
+       removed' := removed + found;
+    }
+
+    method problem4_2(input: string) returns (x: int)
+        decreases *
+    {
+       var grid, length := parseInput(input);
+       x := 0;
+       var found: set<(nat, nat)> := {};
+       var nRemoved, removed := problem4_helper(grid, length, found);
+       while nRemoved > 0 
+         decreases *
+       {
+            nRemoved, removed := problem4_helper(grid, length, removed);
+            // print "\nRemoved ", nRemoved," ", removed;
+       }
+       x := |removed|;
     }
 }
